semantics with effects

coq/Semantics.v
@@ -1,53 +1,93 @@
-(**
-  Master Thesis, Page 10
-  This file contains operational semantics, context semantics and bigstep semantics as well as the definition of normal forms, normality and
-  evaluation
-*)
+(** Master Thesis, Page 10 This file contains operational semantics, context
+  semantics and bigstep semantics as well as the definition of normal forms,
+  normality and evaluation *)
 
 Set Implicit Arguments.
 Require Import Psatz Logic List Classes.Morphisms.
 Import List Notations.
 
-Require Export CBPV.Terms CBPV.Base CBPV.AbstractReductionSystems.
+Require Export CBPV.Terms CBPV.Base.
 Import CommaNotation.
 
+(* Effect axiomatization *)
+
+Axiom eff_idL : forall {e}, add pure e = e .
+Axiom eff_idR : forall {e}, add e pure = e .
+Axiom eff_assoc : forall {e1 e2 e3}, add (add e1 e2) e3 = add e1 (add e2 e3).
+
+#[export] Hint Resolve eff_idL eff_idR eff_assoc : core.
+#[export] Hint Rewrite @eff_idL @eff_idR @eff_assoc : core.
+
+Ltac esimpl := autorewrite with core.
 
 (** * Semantics *)
 
-Reserved Notation "A '≽' B" (at level 80).
-Reserved Notation "A '⇝' B" (at level 80).
+Reserved Notation "A '≽' B '#' phi" (at level 80).
+Reserved Notation "A '⇝' B '#' phi" (at level 80).
+Reserved Notation "A '≻' B '#' phi" (at level 80).
 
 (** ** Primitive Reduction  *)
-Inductive pstep {n: nat}: comp n -> comp n -> Prop :=
+Inductive pstep {n: nat}: comp n -> comp n -> effect -> Prop :=
 | pstepForce (c: comp n):
-    <{c}>! ≽ c
+    <{c}>! ≽ c # pure
 | pstepApp (c: comp (S n)) (c': comp n) v:
-    subst_comp (v..) c = c' -> (lambda c) v ≽ c'
+    subst_comp (v..) c = c' -> (lambda c) v ≽ c' # pure
 | pstepProj (b: bool) (c c1 c2: comp n) :
-    (c = if b then c1 else c2) -> proj b (tuple c1 c2) ≽ c
+    (c = if b then c1 else c2) -> proj b (tuple c1 c2) ≽ c # pure
 | pstepLetin (c: comp (S n)) c' v:
-    subst_comp (v..) c = c' -> $ <- (ret v); c ≽ c'
+    subst_comp (v..) c = c' -> $ <- (ret v); c ≽ c' # pure
 | pstepCaseS v (b: bool) c (c1 c2: comp (S n)):
-    subst_comp (v..) (if b then c1 else c2) = c -> caseS (inj b v) c1 c2 ≽ c
+    subst_comp (v..) (if b then c1 else c2) = c -> caseS (inj b v) c1 c2 ≽ c # pure
 | pstepCaseP v1 v2 (c: comp (S (S n))) c':
-    subst_comp (v2,v1..) c = c' -> caseP (pair v1 v2) c ≽ c'
-| pstepTock :  tock ≽ ret u
-where "A '≽' B" := (pstep A B).
+    subst_comp (v2,v1..) c = c' -> caseP (pair v1 v2) c ≽ c' # pure
+| pstepTock :  tock ≽ ret u # tick
+where "A '≽' B '#' phi" := (pstep A B phi).
 
 
 (** ** Operational Semantics *)
-Inductive step {n: nat}: comp n -> comp n -> Prop :=
-| stepPrimitive (c c': comp n) : c ≽ c' -> c > c'
-| stepApp (c c': comp n) v: c > c' -> c v > c' v
-| stepProj (c c': comp n)  b: c > c' -> proj b c > proj b c'
-| stepLetin (c1 c1': comp n) c2: c1 > c1' -> $ <- c1; c2 > $ <- c1'; c2
-where "A > B" := (step A B).
+Inductive step {n: nat} : comp n -> comp n -> effect -> Prop :=
+| stepPrimitive (c c': comp n) phi : c ≽ c' # phi -> (c ≻ c' # phi)
+| stepApp (c c': comp n) v phi  : c ≻ c' # phi -> c v ≻ c' v # phi
+| stepProj (c c': comp n)  b phi : c ≻ c' # phi -> proj b c ≻ proj b c' # phi
+| stepLetin (c1 c1': comp n) c2 phi: 
+  c1 ≻ c1' # phi -> $ <- c1; c2 ≻ $ <- c1'; c2 # phi
+where "A '≻' B '#' phi" := (step A B phi).
 
-Hint Constructors pstep step.
+#[export] Hint Constructors pstep step : core.
 
-Notation "A >* B" := (star step A B) (at level 60).
-Notation "A >+ B" := (plus step A B) (at level 60).
+Inductive eff_star (X : Type) (R : X -> X -> effect -> Prop) : X -> X -> effect -> Prop :=
+  | eff_starRefl : forall x, eff_star R x x pure
+  | eff_starStep : forall x x' y p1 p2 p, 
+      R x x' p1 
+        -> eff_star R x' y p2 
+        -> add p1 p2 = p
+        -> eff_star R x y p.
 
+Inductive eff_plus (X : Type) (R : X -> X -> effect -> Prop) : X -> X -> effect -> Prop :=
+    eff_plusSingle : forall x y phi, R x y phi -> eff_plus R x y phi 
+  | eff_plusStep : forall x x' y p1 p2 p, 
+      R x x' p1 
+      -> eff_plus R x' y p2 
+      -> add p1 p2 = p
+      -> eff_plus R x y p.
+
+#[export] Hint Constructors eff_star eff_plus : core.
+
+Notation "A >* B # phi " := (eff_star step A B phi) (at level 60).
+Notation "A >+ B # phi" := (eff_plus step A B phi) (at level 60).
+
+Lemma eff_starTrans  (X : Type) (R : X -> X -> effect -> Prop) : 
+  forall x1 x2 p1, 
+    eff_star R x1 x2 p1 
+    -> forall x3 p2 p, eff_star R x2 x3 p2 
+    -> add p1 p2 = p 
+    -> eff_star R x1 x3 p.
+Proof.
+  induction 1; intros; esimpl; subst; eauto.
+  esimpl. auto.
+Qed.
+
+#[export] Hint Resolve eff_starTrans : core.
 
 (** ** Context Semantics *)
 (** Evaluation context *)
@@ -67,33 +107,46 @@ Fixpoint fill {n: nat} (K: ectx) (c: comp n) :=
   end.
 
 (** Context Semantics *)
-Inductive cstep {n: nat}: comp n -> comp n -> Prop :=
-| contextStep C c c' (c'' c''': comp n):
-    c ≽ c' -> fill C c = c'' -> fill C c' = c''' -> c'' ⇝ c'''
-where "A '⇝' B" := (cstep A B).
+Inductive cstep {n: nat}: comp n -> comp n -> effect -> Prop :=
+| contextStep C c c' (c'' c''': comp n) phi :
+    (c ≽ c' # phi) -> fill C c = c'' -> fill C c' = c''' -> (c'' ⇝ c''' # phi)
+where "A '⇝' B '#' phi" := (cstep A B phi).
 
 (** ** Bigstep Semantics *)
-Reserved Notation "A ▷ B" (at level 80).
+Reserved Notation "A ▷ B # phi" (at level 80).
 
-Inductive bigstep {n: nat}: comp n -> comp n -> Prop :=
-| bigstepCu: @cu n ▷ cu
-| bigstepReturn (v: value n) : ret v ▷ ret v
-| bigstepLambda (c: comp (S n)) : lambda c ▷ lambda c
-| bigstepTuple (c1 c2: comp n): tuple c1 c2 ▷ tuple c1 c2
-| bigstepForce (c c': comp n): c ▷ c' -> <{c}>! ▷ c'
-| bigstepApp (c c'': comp n) c' v: c ▷ lambda c' -> subst_comp (v..) c' ▷ c'' -> c v ▷ c''
-| bigstepProj c c' (c1 c2: comp n) (b: bool):
-    c ▷ tuple c1 c2 -> (if b then c1 else c2) ▷ c' -> proj b c ▷ c'
-| bigstepLetin c1 (v: value n) c2 c: c1 ▷ ret v -> subst_comp (v..) c2 ▷ c -> $ <- c1; c2 ▷ c
-| bigstepCaseS c c1 c2 (b: bool) (v: value n):
-  subst_comp (v..) (if b then c1 else c2) ▷ c -> caseS (inj b v) c1 c2 ▷ c
-| bigstepCaseP c c' (v1 v2: value n):
-    subst_comp (v2,v1..) c ▷ c' -> caseP (pair v1 v2) c ▷ c'
+Inductive bigstep {n: nat}: comp n -> comp n -> effect -> Prop :=
+| bigstepCu: @cu n ▷ cu # pure
+| bigstepReturn (v: value n) : ret v ▷ ret v # pure 
+| bigstepLambda (c: comp (S n)) : lambda c ▷ lambda c # pure
+| bigstepTuple (c1 c2: comp n): tuple c1 c2 ▷ tuple c1 c2 # pure
+| bigstepForce (c c': comp n) phi: c ▷ c' # phi -> <{c}>! ▷ c' # phi
+| bigstepApp (c c'': comp n) c' v phi1 phi2  phi: 
+  c ▷ lambda c' # phi1 
+  -> subst_comp (v..) c' ▷ c'' # phi2
+  -> add phi1 phi2 = phi
+  -> c v ▷ c'' # phi
+| bigstepProj c c' (c1 c2: comp n) (b: bool) phi1 phi2 phi:
+    c ▷ tuple c1 c2 # phi1 
+    -> (if b then c1 else c2) ▷ c' # phi2 
+    -> add phi1 phi2 = phi
+    -> proj b c ▷ c' # phi
+| bigstepLetin c1 (v: value n) c2 c phi1 phi2 phi: 
+  c1 ▷ ret v #phi1 
+  -> subst_comp (v..) c2 ▷ c # phi2
+  -> add phi1 phi2 = phi
+  -> $ <- c1; c2 ▷ c # phi
+| bigstepCaseS c c1 c2 (b: bool) (v: value n) phi:
+  subst_comp (v..) (if b then c1 else c2) ▷ c # phi
+  -> caseS (inj b v) c1 c2 ▷ c # phi
+| bigstepCaseP c c' (v1 v2: value n) phi:
+    subst_comp (v2,v1..) c ▷ c' # phi
+    -> caseP (pair v1 v2) c ▷ c' # phi
 | bigstepTock :
-    tock ▷ ret u
-where "A ▷ B" := (bigstep A B).
+    tock ▷ ret u # tick
+where "A ▷ B  # phi" := (bigstep A B phi).
 
-Hint Constructors bigstep.
+#[export] Hint Constructors bigstep : core.
 
 (** ** Normal Form *)
 Inductive nf {n: nat}: comp n -> Prop :=
@@ -102,21 +155,28 @@ Inductive nf {n: nat}: comp n -> Prop :=
 | nfTup c1 c2: nf (tuple c1 c2)
 | nfRet v: nf (ret v).
 
-Hint Constructors nf.
+#[export] Hint Constructors nf : core.
 
 
 (** ** Evaluation *)
-Definition eval {n: nat} (c c': comp n) := c >* c' /\ nf c'.
-Hint Transparent  eval.
+Definition eval {n: nat} (c c': comp n) phi := c >* c' # phi /\ nf c'.
+#[export] Hint Transparent eval : core.
 
 (** ** Properties *)
 
-Instance proper_letin {n: nat}: Proper (star step ++> eq ++> star step) (@letin n).
+(*
+Definition eff_respectful :=
+  fun {A:Type}
+    (R : A -> A -> effect -> Prop) (R' : A -> A -> effect -> Prop) (f g : A -> A)
+  => (forall (x y : A) phi, R x y phi -> R' (f x) (g y) phi).
+
+Notation "R +++> R'" := (eff_respectful R R') (at level 55).
+
+Instance proper_letin {n: nat}{phi: effect} : Proper (eff_star step +++> (fun c1 c2 phi => eq c1 c2) +++> eff_star step) (@letin n).
 Proof.
-  intros c1 c1' H ? c2 ->.
+  intros c1 c1' H ? c2 ->. unfold eff_star_step.
   induction H; eauto.
 Qed.
-
 
 Instance proper_app {n: nat}: Proper (star step ++> eq ++> star step) (@app n).
 Proof.
@@ -130,9 +190,34 @@ Proof.
   intros ? i -> c c' H.
   induction H; eauto.
 Qed.
+*)
+
+Lemma step_letin {n:nat} (c1 c1' : comp n) (c2 : comp (S n)) phi : 
+  eff_star step c1 c1' phi ->
+  eff_star step (letin c1 c2) (letin c1' c2) phi.
+Proof.
+  induction 1; eauto. 
+Qed.
 
 
-Hint Resolve proper_letin proper_app proper_proj.
+Lemma step_app {n:nat} (c1 c1' : comp n) (v : value n) phi : 
+  eff_star step c1 c1' phi ->
+  eff_star step (app c1 v) (app c1' v) phi.
+Proof.
+  induction 1; eauto. 
+Qed.
+
+Lemma step_proj {n:nat} (c1 c1' : comp n) b phi : 
+  eff_star step c1 c1' phi ->
+  eff_star step (proj b c1) (proj b c1') phi.
+Proof.
+  induction 1; eauto. 
+Qed.
+
+
+#[export] Hint Resolve step_letin step_app step_proj : core.
+#[export] Hint Rewrite @step_letin @step_app @step_proj : core.
+
 
 (** Reduction tactic for beta reduction step *)
 Ltac reduce := econstructor 2; [ solve [eauto] | cbn ].
@@ -140,14 +225,25 @@ Ltac reduce := econstructor 2; [ solve [eauto] | cbn ].
 
 
 (** Substitution Primitive Step *)
-Lemma pstep_subst m n (C1 C2: comp m) (f: fin m -> value n):
-  C1 ≽ C2 -> subst_comp f C1 ≽ subst_comp f C2.
+Lemma pstep_subst m n (C1 C2: comp m) (f: fin m -> value n) phi:
+  C1 ≽ C2 # phi -> subst_comp f C1 ≽ subst_comp f C2 # phi.
 Proof.
   intros H; inv H; cbn; constructor; try destruct b; asimpl; reflexivity.
 Qed.
 
 (** The operational semantic we defined is functional *)
-Lemma step_functional {n: nat} (c1 c2 c2': comp n) : c1 > c2 -> c1 > c2' -> c2 = c2'.
+Lemma step_functional {n: nat} (c1 c2 c2': comp n) phi1 phi2 : 
+  c1 ≻ c2 # phi1 -> c1 ≻ c2' # phi2  -> c2 = c2'.
+Proof.
+  induction 1 in c2' |-*; intros H1; inv H1.
+  1: inv H; inv H0; reflexivity.
+  all: try (inv H; inv H0; inv H).
+  all: try (inv H0; inv H; inv H0).
+  all: firstorder congruence.
+Qed.
+
+Lemma step_functional_eff {n: nat} (c1 c2 c2': comp n) phi1 phi2 : 
+  c1 ≻ c2 # phi1 -> c1 ≻ c2' # phi2  -> phi1 = phi2.
 Proof.
   induction 1 in c2' |-*; intros H1; inv H1.
   1: inv H; inv H0; reflexivity.
@@ -157,6 +253,7 @@ Proof.
 Qed.
 
 
+(*
 Lemma confluence_steps (n: nat):
   confluent (@step n).
 Proof.
@@ -168,12 +265,12 @@ Proof.
 Qed.
 
 Hint Resolve confluence_steps.
-
+*)
 
 
 
 (** The operational semantic and the context semantic agree *)
-Lemma step_equiv {n: nat} (c c': comp n): c > c' <->  c ⇝ c'.
+Lemma step_equiv {n: nat} (c c': comp n) phi : c ≻ c' # phi <->  c ⇝ c' # phi.
 Proof.
   split.
   - induction 1.
@@ -186,145 +283,170 @@ Proof.
 Qed.
 
 
-
 (** The bigstep semantic is sound w.r.t the operational semantic *)
-Lemma bigstep_soundness {n: nat} (c c': comp n): c ▷ c' -> c >* c'.
+Lemma bigstep_soundness {n: nat} (c c': comp n) phi: c ▷ c' # phi -> c >* c' # phi.
 Proof.
   induction 1; eauto.
-  - rewrite IHbigstep1; reduce; rewrite IHbigstep2; reflexivity.
-  - rewrite IHbigstep1; reduce; assumption.
-  - rewrite IHbigstep1; reduce; rewrite IHbigstep2; reflexivity.
+  - apply step_app with (v:=v) in IHbigstep1.
+    eapply eff_starTrans; eauto.
+  - apply step_proj with (b := b) in IHbigstep1.
+    eapply eff_starTrans; eauto.
+  - apply step_letin with (c2 := c2) in IHbigstep1.
+    eauto.
 Qed.
 
 
-(** The bigstep semantic is closed under expasion by the operational semantics *)
-Lemma bigstep_primitive_cons {n: nat} (c c' c'': comp n): c ≽ c' -> c' ▷ c'' -> c ▷ c''.
+(** The bigstep semantic is closed under expansion by the operational semantics *)
+Lemma bigstep_primitive_cons {n: nat} (c c' c'': comp n) phi1 phi2: 
+  c ≽ c' # phi1
+  -> c' ▷ c'' # phi2 
+  -> c ▷ c''  # add phi1 phi2.
 Proof.
-  intros H; inv H; intros H; try econstructor; eauto. inv H; eauto.
+  intros H; inv H; try intros H; esimpl; try econstructor; eauto. 
+  inv H; esimpl; eauto.
 Qed.
 
 
-Lemma bigstep_cons {n: nat} (c c' c'': comp n): c > c' -> c' ▷ c'' -> c ▷ c''.
+Lemma bigstep_cons {n: nat} (c c' c'': comp n) phi1 phi2 : 
+  c ≻ c' # phi1 -> c' ▷ c'' # phi2 -> c ▷ c'' # add phi1 phi2.
 Proof.
-  induction 1 in c'' |-*.
+  induction 1 in c'', phi2 |-*.
   1: now apply bigstep_primitive_cons.
-  all: intros H1; inv H1; eauto.
+  all: intros H1; inv H1; esimpl; eauto.
 Qed.
 
-Lemma bigstep_prepend {n: nat} (c c' c'': comp n): c >* c' -> c' ▷ c'' -> c ▷ c''.
+Lemma bigstep_prepend {n: nat} (c c' c'': comp n) phi1 phi2:  
+  c >* c' # phi1 -> c' ▷ c'' # phi2 -> c ▷ c'' # (add phi1 phi2).
 Proof.
-  induction 1 in c'' |-*; intros; eauto using bigstep_cons.
+  induction 1 in c'', phi2 |-*; intros; subst; esimpl; eauto using bigstep_cons.
 Qed.
 
-Hint Resolve bigstep_cons bigstep_prepend.
+#[export] Hint Resolve bigstep_cons bigstep_prepend : core.
 
 
 
 (** The bigstep semantic is functional *)
-Lemma bigstep_functional {n: nat} (c1 c2 c2': comp n) : c1 ▷ c2 -> c1 ▷ c2' -> c2 = c2'.
+Lemma bigstep_functional {n: nat} (c1 c2 c2': comp n) phi1 phi2 : 
+  c1 ▷ c2 # phi1 -> c1 ▷ c2' # phi2 -> c2 = c2'.
 Proof.
-  induction 1 in c2' |-*; intros H1; inv H1; eauto.
-  all: specialize (IHbigstep1 _ H4); injection IHbigstep1; repeat intros ->; apply IHbigstep2; eauto.
+  induction 1 in c2' , phi2 |-*; intros h1; inv h1; eauto.
+  all: specialize (IHbigstep1 _ _ H4); injection IHbigstep1; repeat intros ->; eapply IHbigstep2; eauto.
 Qed.
 
+Definition eff_Normal {X : Type} (R : X -> X -> effect -> Prop) (x : X) :=
+  forall (y : X) phi,  ~ R x y phi.
+
 (** Normal forms are normal *)
-Lemma nf_normal {n: nat} (c: comp n) : nf c -> Normal step c.
-Proof. intros [] c' H; inv H; inv H0. Qed.
+Lemma nf_normal {n: nat} (c: comp n) : nf c -> eff_Normal step c.
+Proof. intros [] c' eff H; inv H; inv H0. Qed.
 
 (** Terms bigstep evaluate to normal forms *)
-Lemma bigstep_normal {n: nat} (c c': comp n): c ▷ c' -> nf c'.
+Lemma bigstep_normal {n: nat} (c c': comp n) eff : c ▷ c' # eff -> nf c'.
 Proof.
   induction 1; eauto.
 Qed.
 
 (** Normal forms bigstep evaluate *)
-Lemma normal_bigstep {n: nat} (c: comp n): nf c -> c ▷ c.
+Lemma normal_bigstep {n: nat} (c: comp n): nf c -> c ▷ c # pure.
 Proof.
   intros []; eauto.
 Qed.
 
+
 (** Bigstep evaluation is evaluation *)
-Lemma eval_bigstep {n: nat} (c c': comp n): eval c c' <-> c ▷ c'.
+Lemma eval_bigstep {n: nat} (c c': comp n) phi : eval c c' phi<-> c ▷ c' # phi.
 Proof.
   split.
-  - intros [H1 H2]; induction H1; eauto using normal_bigstep, bigstep_cons.
+  - intros [H1 H2]; induction H1; subst; eauto using normal_bigstep, bigstep_cons.
   - intros H; split; eauto using bigstep_normal, bigstep_soundness.
 Qed.
 
 
-
-Lemma ectx_decompose {n: nat} (K : @ectx n) c c':
-  fill K c ▷ c' -> exists c'', c ▷ c'' /\ fill K c'' ▷ c'.
+Lemma ectx_decompose {n: nat} (K : @ectx n) c c' phi:
+  fill K c ▷ c' # phi -> exists c'' phi1 phi2, c ▷ c'' # phi1  /\ fill K c'' ▷ c' # phi2 /\ phi = add phi1 phi2.
 Proof.
-  induction K in c, c' |-*; cbn; intros H.
-  1: eexists; intuition; eauto; induction H; eauto.
-  all: inv H; edestruct IHK; eauto; intuition.
-  all: eexists; intuition; eauto.
+  induction K in c, c', phi |-*; cbn; intros H.
+  1: { exists c'. exists phi. exists pure. repeat split; eauto using bigstep_normal, normal_bigstep. }
+  all: inv H; edestruct IHK as [c'' [phi1' [phi2' h]]]; eauto; intuition.
+  all: eexists; eexists; eexists.
+  split. eauto. split. eauto. subst. esimpl. reflexivity.
+  split. eauto. split. eauto. subst. esimpl. reflexivity.
+  split. eauto. split. eauto. subst. esimpl. reflexivity.
 Qed.
 
-Lemma ectx_compose {n: nat} (K : @ectx n) c c' c'':
-  c ▷ c' -> fill K c' ▷ c'' -> fill K c ▷ c''.
+Lemma ectx_compose {n: nat} (K : @ectx n) c c' c'' phi1 phi2:
+  c ▷ c' # phi1 -> fill K c' ▷ c'' # phi2  -> fill K c ▷ c'' # add phi1 phi2.
 Proof.
   intros H1 H2.
   eapply eval_bigstep in H1.
   eapply eval_bigstep in H2.
   eapply eval_bigstep.
   unfold eval in *; intuition.
-  rewrite <-H1.
+  eapply eff_starTrans with (x2 := fill K c'); eauto.
   clear H0 H3 H1; induction K; cbn in *; eauto;
     now rewrite IHK.
 Qed.
 
+Definition eff_evaluates := fun (X : Type) (R : X -> X -> effect -> Prop) (s t : X) phi => 
+                             eff_star R s t phi /\ eff_Normal R t.
 
-
-Lemma eval_evaluates n (c c': comp n):
-  evaluates step c c' -> nf c' -> eval c c'.
+Lemma eval_evaluates n (c c': comp n) phi:
+  eff_evaluates step c c' phi -> nf c' -> eval c c' phi.
 Proof.
   split; eauto. destruct H; eauto. 
 Qed.
 
-Lemma steps_nf_eval n (c c': comp n):
-    c >* c' -> nf c' ->  eval c c'.
+Lemma steps_nf_eval n (c c': comp n) phi:
+    c >* c' # phi -> nf c' ->  eval c c' phi.
 Proof.
   split; eauto.
 Qed.
 
 
-Lemma steps_bigstep n (c c': comp n):
-    c >* c' -> nf c' -> c ▷ c'.
+Lemma steps_bigstep n (c c': comp n) phi:
+    c >* c' # phi -> nf c' -> c ▷ c' # phi.
 Proof.
   intros; eapply eval_bigstep, steps_nf_eval; eauto.
 Qed.
 
 
 (** Star Steps are functional if the term steps to a term in normal form *)
-Lemma starstep_functional_nf {n: nat} (c c1 c2: comp n):
-   c >* c1 -> c >* c2 -> nf c1 -> nf c2 -> c1 = c2.
+Lemma starstep_functional_nf {n: nat} (c c1 c2: comp n) phi1 phi2 :
+   c >* c1 # phi1 -> c >* c2 # phi2 -> nf c1 -> nf c2 -> c1 = c2.
 Proof.
   intros; eapply bigstep_functional; eapply eval_bigstep; unfold eval; split; eauto.
 Qed.
 
+Inductive eff_SN (X : Type) (R : X -> X -> effect -> Prop) : X -> Prop :=  
+  eff_SNC : forall (x : X), (forall (y : X) phi, R x y phi -> eff_SN R y) -> eff_SN R x.
+
 
 (** Strong Normaliation is closed under expansion *)
-Lemma normalizing_extension {n: nat} (c c': comp n):
-  c >* c' -> SN step c' -> SN step c.
+Lemma normalizing_extension {n: nat} (c c': comp n) phi :
+  c >* c' # phi -> eff_SN step c' -> eff_SN step c.
 Proof.
   induction 1.
   - now intros.
-  - intros H1 % IHstar. constructor. intros x'' H2.
+  - intros h1 % IHeff_star. constructor. intros x'' p3 h2.    
     enough (x' = x'') as -> by assumption.
-    eapply step_functional; eassumption.
+    eapply step_functional; eassumption. 
 Qed.
+
+Definition eff_Normal_eff_SN := 
+fun (X : Type) (R : X -> X -> effect -> Prop) (x : X) (H : eff_Normal R x) => 
+  eff_SNC x (fun (y : X) phi (H1 : R x y phi) => False_ind (eff_SN R y) (H y phi H1)).
 
 (** Bigstep Semantics implies termination *)
-Lemma bigstep_sn' {n: nat} (c c': comp n) : c ▷ c' -> SN step c'.
+Lemma bigstep_sn' {n: nat} (c c': comp n) phi : c ▷ c' # phi -> eff_SN step c'.
 Proof.
-  intros H % eval_bigstep; destruct H; now apply Normal_SN, nf_normal.
+  intros H % eval_bigstep; destruct H; now apply eff_Normal_eff_SN, nf_normal.
 Qed.
 
 
-Lemma bigstep_sn {n: nat} (c c': comp n) : c ▷ c' -> SN step c.
+Lemma bigstep_sn {n: nat} (c c': comp n) phi : c ▷ c' # phi -> eff_SN step c.
 Proof.
   intros H; eapply normalizing_extension; [| eapply bigstep_sn'; eassumption].
-  enough (eval c c') by firstorder. now apply eval_bigstep.
+  enough (eval c c' phi). 
+  eapply bigstep_soundness.  eauto. 
+  rewrite -> eval_bigstep. auto.
 Qed.
